Update lagrange to work with modules.

src/Field.ec
@@ -40,28 +40,26 @@ op (^) (x : FieldR.F) (k : int) = FieldR.exp x k axiomatized by RexpE.
 require import AllCore Int IntDiv ZModP.
 require import Constants.
 
-print r.
-
 clone include ZModField  with 
-  op p <- r 
+  op p <- R 
   rename "zmod" as "Fr"
   rename "ZModp" as "Zr"
   proof prime_p by apply prime_r.
    
 op (^) (x : Fr) (k : int) = exp x k axiomatized by expE.
 
-op omegaFr = inFr omega axiomatized by omegaFrE.
-op domain_sizeFr = inFr domain_size axiomatized by domain_sizeFrE.
+op OMEGAFr = inFr OMEGA axiomatized by omegaFrE.
+op DOMAIN_SIZEFr = inFr DOMAIN_SIZE axiomatized by domain_sizeFrE.
 
-lemma omega_eq_omegaFr : asint omegaFr = omega.
+lemma omega_eq_omegaFr : asint OMEGAFr = OMEGA.
 proof.
-  rewrite omegaFrE /asint /inFr; have ->: omega %% r = omega by smt.
+  rewrite omegaFrE /asint /inFr; have ->: OMEGA %% R = OMEGA by smt.
   rewrite Sub.insubdK //; smt.
 qed.
 
-lemma domain_eq_domainFr : asint domain_sizeFr = domain_size.
+lemma domain_eq_domainFr : asint DOMAIN_SIZEFr = DOMAIN_SIZE.
 proof.
-  rewrite domain_sizeFrE /asint /inFr; have ->: domain_size %% r = domain_size by smt.
+  rewrite domain_sizeFrE /asint /inFr; have ->: DOMAIN_SIZE %% R = DOMAIN_SIZE by smt.
   rewrite Sub.insubdK //; smt.
 qed.
 >>>>>>> 207ac17 (refined specs.)
