src/specs/evaluateLagrangePolyOutOfDomain.ec
@@ -1,21 +1,55 @@
 pragma Goals:printall.
 
-require import AllCore Int IntDiv Wheels Constants Field.
+require import AllCore Int IntDiv Constants Field.
+
+op lagrangeM (i z : int) : int =
+  let omi  = (OMEGA^i) %% R in
+  let zd1  = (z^DOMAIN_SIZE - 1) %% R in
+  let num  = (omi * zd1) %% R in
+  let invd = ((DOMAIN_SIZE * (z - omi)) %% R)^(R - 2) %% R in
+  (num * invd) %% R.
+
+op lagrangeH (i : int) (z : Fr) : Fr =
+  (OMEGAFr^i * (z^DOMAIN_SIZE - one)) / (DOMAIN_SIZEFr * (z - OMEGAFr^i)).
+
+module EvaluateLagrangePolyOutOfDomain = {
+  proc mid(i: int, z: int) : int option = {
+    var r;
+    
+    if((z^DOMAIN_SIZE - 1)%%R = 0) {
+      r <- None;
+    } else {
+      r <- Some (lagrangeM i z);
+    }  
+    return r;
+  }
+
+  proc high(i: int, z: Fr) : Fr option = {
+    var r;
+    
+    if((z^DOMAIN_SIZE - one) = zero) {
+      r <- None;
+    } else {
+      r <- Some (lagrangeH i z);
+    }  
+    return r;
+  }
+}.
 
 (* Mid-level *)
-op evalLagrange_Mspec_res (i z rs : int) : bool =
-  let omi  = (omega^i) %% r in
-  let zd1  = (z^domain_size - 1) %% r in
-  let num  = (omi * zd1) %% r in
-  let invd = ((domain_size * (z - omi)) %% r)^(r - 2) %% r in
-  rs = (num * invd) %% r.
+(* op evalLagrange_Mspec_res (i z rs : int) : bool = *)
+(*   let omi  = (omega^i) %% r in *)
+(*   let zd1  = (z^domain_size - 1) %% r in *)
+(*   let num  = (omi * zd1) %% r in *)
+(*   let invd = ((domain_size * (z - omi)) %% r)^(r - 2) %% r in *)
+(*   rs = (num * invd) %% r. *)
 
-op evalLagrange_Mspec (i z rs : int) : bool =
-  (!((z^domain_size - 1) %% r = 0) => !Primops.reverted /\ evalLagrange_Mspec_res i z rs)
-  /\
-  ((z^domain_size - 1) %% r = 0 => Primops.reverted).
+(* op evalLagrange_Mspec (i z rs : int) : bool = *)
+(*   (!((z^domain_size - 1) %% r = 0) => !Primops.reverted /\ evalLagrange_Mspec_res i z rs) *)
+(*   /\ *)
+(*   ((z^domain_size - 1) %% r = 0 => Primops.reverted). *)
 
-(* High-level *)
-op evalLagrange_Hspec (i : int) (z rs : Fr) : bool =
-  !(z^domain_size - one = zero) =>
-  rs = (omegaFr^i * (z^domain_size - one)) / (domain_sizeFr * (z - omegaFr^i)).
+(* (* High-level *) *)
+(* op evalLagrange_Hspec (i : int) (z rs : Fr) : bool = *)
+(*   !(z^domain_size - one = zero) => *)
+(*   rs = (omegaFr^i * (z^domain_size - one)) / (domain_sizeFr * (z - omegaFr^i)). *)
